\documentclass{article}
\usepackage{epsfig}
\pagestyle{empty}
\begin{document}
\[ r_h(t) = b_h s(t - \tau_h) e^{j2\pi f_{D,h}} \]
\pagebreak

$f_C$
\pagebreak

$\sigma_{\text{RCS},h}$
\pagebreak

$d_h$
\pagebreak

$c_0$
\pagebreak

\[ b_h = \sqrt{\frac{c_0^2 \sigma_{\text{RCS},h}}{(4\pi)^3 d_h^4 f_C^2}} \]
\pagebreak

$\tau_h$
\pagebreak

\[ \tau_h = 2\frac{d_h}{c_0} \]
\pagebreak

$f_{D,h}$
\pagebreak

\[ f_{D,h} = 2\frac{v_{\text{rel},h}{c_0} f_C \]
\pagebreak

\[ r(t) = \sum_{h=0}^{H-1} r_h(t) \]
\pagebreak

\end{document}
